new/golang/theory/interface.v
@@ -5,10 +5,10 @@ From New.golang.defn Require Import interface globals.
 Section wps.
 Context `{sem: ffi_semantics} `{!ffi_interp ffi} `{!heapGS Σ}.
 
-Global Instance wp_interface_get (i : interface.t) (method : go_string) pkg_name type_name :
-  PureWp (i.(interface.opt_pkg_type_name) = Some (pkg_name, type_name))
+Global Instance wp_interface_get (i : interface.t) (method : go_string) pkg_name type_name v :
+  PureWp (i = interface.mk pkg_name type_name v)
     (interface.get #method #i)
-    (method_call #pkg_name #type_name #method i.(interface.v)).
+    (method_call #pkg_name #type_name #method v).
 Proof.
   iIntros (?????) "Hwp".
   rewrite [in #i]to_val_unseal interface.get_unseal.
@@ -17,11 +17,37 @@ Proof.
 Qed.
 
 Global Instance wp_interface_make (v : val) pkg_name type_name :
-  PureWp (True) (interface.make #pkg_name #type_name v) #(interface.mk v (Some (pkg_name, type_name))).
+  PureWp (True) (interface.make #pkg_name #type_name v) #(interface.mk pkg_name type_name v).
 Proof.
   iIntros (?????) "Hwp".
   rewrite [in #(_ : interface.t)]to_val_unseal interface.make_unseal.
   wp_call_lc "?". wp_pures. by iApply "Hwp".
+Qed.
+
+Global Instance wp_interface_eq_nil_r (i : interface.t) :
+  PureWp (True) (interface.eq #i #interface.nil) #(bool_decide (i = interface.nil)).
+Proof.
+  pose proof wp_eq_val.
+  iIntros (?????) "Hwp".
+  rewrite to_val_unseal.
+  wp_call_lc "?".
+  rewrite to_val_unseal.
+  destruct i as [|].
+  - wp_pures. wp_pures. rewrite bool_decide_false //. by iApply "Hwp".
+  - wp_pures. rewrite bool_decide_true //. by iApply "Hwp".
+Qed.
+
+Global Instance wp_interface_eq_nil_l (i : interface.t) :
+  PureWp (True) (interface.eq #interface.nil #i) #(bool_decide (interface.nil = i)).
+Proof.
+  pose proof wp_eq_val.
+  iIntros (?????) "Hwp".
+  rewrite to_val_unseal.
+  wp_call_lc "?".
+  rewrite to_val_unseal.
+  destruct i as [|].
+  - wp_pures. wp_pures. rewrite bool_decide_false //. by iApply "Hwp".
+  - wp_pures. rewrite bool_decide_true //. by iApply "Hwp".
 Qed.
 
 End wps.
